SPLean/Theories/NWO.lean
@@ -1,0 +1,50 @@
+import Lean.Elab.Tactic
+import Qq
+
+import SPLean.Theories.HProp
+import SPLean.Common.Util
+
+
+-- open hprop_scope
+open Lean Lean.Expr Lean.Meta Qq
+open Lean Elab Command Term Meta Tactic
+
+/- [nwo] (No Wand Out) tactic implementation -/
+inductive hprop : Type where
+  | sep : List hprop -> hprop
+  | pure : Expr -> hprop
+  | emp : hprop
+  | wand : hprop -> hprop -> hprop
+  | exists : Name -> Expr -> hprop -> hprop
+deriving Inhabited
+
+partial def Lean.Expr.toHprop (e : Expr) : hprop :=
+  match_expr e with
+  | HStar.hStar _ _ _ _ h₁ h₂ => hprop.sep (go h₁ ++ go h₂)
+  | HWand.hWand _ _ _ _ h₁ h₂ => hprop.wand h₁.toHprop h₂.toHprop
+  | hpure p => hprop.pure p
+  | hempty => hprop.emp
+  | hexists _ j =>
+    match j.consumeMData with
+    | forallE n tp bd _ => hprop.exists n tp bd.toHprop
+    | _ => panic! s!"{j} is not a valid existential quantifier"
+  | _ => panic! s!"{e} is not handled yet"
+  where
+go (e : Expr) : List hprop :=
+  match_expr e with
+  | HStar.hStar _ _ _ _ h₁ h₂ => go h₁ ++ go h₂
+  | _ => [e.toHprop]
+
+structure NWOState where
+  pures : List Expr
+  ----
+  hla : hprop
+  hlw : hprop
+  hlt : hprop
+  ----
+  hra : hprop
+  hrw : hprop
+  hrt : hprop
+
+-- Get the symbolic state from the goal
+def getEntailment : TacticM NWOState := sorry
